revise

chap2_4revisedScript.sml
@@ -8,25 +8,24 @@ open set_relationTheory;
 open finite_mapTheory;
 open chap1Theory;
 
+open folModelsTheory
+open folLangTheory
+
 
 val _ = ParseExtras.tight_equality()
 
 val _ = new_theory "chap2_4revised";
 
-val _ = Datatype`
-        folmodel = <| domain : 'a set ;
-	              consts : num |-> 'a;
-	              fnsyms : num -> 'a list -> 'a;
-		      predsyms : 'p -> 'a -> bool;
-		      relsyms : 'r -> 'a -> 'a -> bool;
-		      |>`;
-
 val mm2folm_def = Define`
-  mm2folm M = <| domain := M.frame.world ;
-                 consts := FEMPTY;
-                 fnsyms := \x y. ARB;
-		 predsyms := \p w. (w IN M.frame.world /\ M.valt p w);
-		 relsyms := \ (u:unit) w1 w2. (M.frame.rel w1 w2 /\ w1 IN M.frame.world /\ w2 IN M.frame.world) |>`;
+  mm2folm M = <| Dom := M.frame.world ;
+                 Fun := \n args. CHOICE (M.frame.world);
+		 Pred := \p zs. 
+                            case zs of
+                              | [w] => w IN M.frame.world /\ M.valt p w
+                              | [w1;w2] => p = 0 ∧ M.frame.rel w1 w2 ∧ 
+                                           w1 IN M.frame.world /\ w2 IN M.frame.world
+                              |  _ => F 
+              |>`;
 
 val expansion_def = Define`
   expansion M0 A M <=> A SUBSET M0.domain /\
@@ -36,90 +35,61 @@ val expansion_def = Define`
 		       M = M0 with consts := FUNION M0.consts (FUN_FMAP f ns)`;
                        
 
-val _ = Datatype`
-        fterm = fVar num
-	       | fConst num (fterm list) ;
-	fform = fRrel 'r fterm fterm
-	       | fPrel 'p fterm
-	       | fDISJ fform fform
-	       | fNOT fform
-	       | fEXISTS num fform
-	       | fEQ fterm fterm`; 
-
-val fAND_def = Define`
-  fAND ff1 ff2 = fNOT (fDISJ (fNOT ff1) (fNOT ff2))`;
 
 
-val fIMP_def = Define`
-  fIMP ff1 ff2 = fDISJ (fNOT ff1) ff2`;
+val _ = overload_on ("fEXISTS", “folLang$Exists”);
+val _ = overload_on ("fDISJ", “folLang$Or”);
+val _ = overload_on ("fAND", “folLang$And”);
+val _ = overload_on ("fNOT", “folLang$Not”);
+val _ = overload_on ("fFALSE", “folLang$False”);
+val _ = overload_on ("fP", “λp t. Pred p [t]”);
+val _ = overload_on ("fR", “λw1 w2. Pred 0 [w1; w2]”);
+val _ = overload_on ("fV", “folLang$V”);
 
+Theorem feval_def = holds_def
+Theorem fAND_def = And_def
 
-val tvars_def = Define`
-  tvars (fVar a) = {a} /\
-  tvars (fConst a l) = {}`;
+Definition ST_def[simp]:
+  (ST x (VAR p) = fP p (fV x)) /\
+  (ST x (FALSE) = fFALSE) /\
+  (ST x (NOT phi) = fNOT (ST x phi)) /\
+  (ST x (DISJ phi psi) = fDISJ (ST x phi) (ST x psi)) /\
+  (ST x (DIAM phi) =
+     fEXISTS (x + 1) (fAND (fR (fV x) (fV (x + 1))) (ST (x + 1) phi)))
+End
 
-val fvars_def = Define`
-  fvars (fRrel a t1 t2) = tvars t1 ∪ tvars t2 /\
-  fvars (fPrel a t) = tvars t /\
-  fvars (fDISJ ff1 ff2) = (fvars ff1) ∪ (fvars ff2) /\
-  fvars (fNOT ff) = fvars ff /\
-  fvars (fEXISTS n ff) = n INSERT (fvars ff) /\
-  fvars (fEQ t1 t2) = tvars t1 ∪ tvars t2`;
+Definition fsatis_def:
+  fsatis M σ fform <=> valuation M σ ∧ feval M σ fform
+End
 
-
-
-
-val ST_def = Define`
-  (ST x (u:unit) (VAR p) <=> fPrel p (fVar x)) /\
-  (ST x u (FALSE) <=> fNOT (fEQ (fVar x) (fVar x))) /\
-  (ST x u (NOT phi) <=> fNOT (ST x u phi)) /\
-  (ST x u (DISJ phi psi) <=> fDISJ (ST x u phi) (ST x u psi)) /\
-  (ST x u (DIAM phi) <=> fEXISTS (x + 1) (fAND (fRrel u (fVar x) (fVar (x + 1))) (ST (x + 1) u phi)))`;
-
-
-(* val interpret_def = Define`
-  interpret M σ (fVar n) = σ n /\
-  interpret M σ (fConst n) = M.consts ' n`;
-
-
-val feval_def = Define`
-  feval M σ (fPrel p t) = M.predsyms p (interpret M σ t) /\
-  feval M σ (fRrel (u:unit) t1 t2) = M.relsyms u (interpret M σ t1) (interpret M σ t2) /\
-  feval M σ (fDISJ f1 f2) = (feval M σ f1 \/ feval M σ f2) /\
-  feval M σ (fNOT f) = ¬(feval M σ f) /\
-  feval M σ (fEXISTS n f) = (?x. x IN M.domain /\ feval M ((n=+x)σ) f) /\
-  feval M σ (fEQ t1 t2) = (interpret M σ t1 = interpret M σ t2)`;
-
-
-
-val fsatis_def = Define`
-  fsatis M σ fform <=> (IMAGE σ univ(:num)) SUBSET M.domain /\
-                       feval M σ fform`;
+(*
+val _ = overload_on ("feval", ``holds``)
+*)
 
 
 val prop_2_47_i = store_thm(
   "prop_2_47_i",
   ``!M w:'b phi σ x. (IMAGE σ univ(:num)) SUBSET M.frame.world
-                       ==> (satis M (σ x) phi <=> fsatis (mm2folm M) σ (ST x (u:unit) phi))``,
+                       ==> (satis M (σ x) phi <=> fsatis (mm2folm M) σ (ST x phi))``,
   Induct_on `phi` >> rw[] (* 5 *)
   >- (rw[feval_def,ST_def,fsatis_def] >> eq_tac >> rw[] (* 3 *)
-     >- fs[mm2folm_def]
-     >- (fs[satis_def] >> rw[interpret_def] >> fs[mm2folm_def,IN_DEF])
+     >- (fs[mm2folm_def,valuation_def,IMAGE_DEF,SUBSET_DEF] >> metis_tac[])
+     >- (fs[satis_def] >> rw[termval_def] >> fs[mm2folm_def,IN_DEF])
      >- (rw[satis_def] >- (fs[IMAGE_DEF,SUBSET_DEF] >> metis_tac[])
-                      >- (fs[interpret_def] >> fs[mm2folm_def,IN_DEF])))
+                       >- (fs[termval_def] >> fs[mm2folm_def,IN_DEF])))
   >- (rw[satis_def,feval_def,ST_def,fsatis_def] >> metis_tac[])
   >- (rw[satis_def,feval_def,ST_def,fsatis_def])
   >- (rw[satis_def,feval_def,ST_def,fsatis_def] >> eq_tac >> rw[] (* 5 *)
-     >- fs[mm2folm_def]
-     >- fs[mm2folm_def]
-     >- fs[mm2folm_def]
+     >- (fs[mm2folm_def,valuation_def,IMAGE_DEF,SUBSET_DEF] >> metis_tac[])
+     >- (fs[mm2folm_def,valuation_def,IMAGE_DEF,SUBSET_DEF] >> metis_tac[])
+     >- (fs[mm2folm_def,valuation_def,IMAGE_DEF,SUBSET_DEF] >> metis_tac[])
      >- rw[]
      >- (fs[IMAGE_DEF,SUBSET_DEF] >> metis_tac[]))
   >- (rw[satis_def,feval_def,ST_def,fsatis_def] >> eq_tac >> rw[] (* 4 *)
-     >- fs[mm2folm_def]
+     >- (fs[mm2folm_def,valuation_def,IMAGE_DEF,SUBSET_DEF] >> metis_tac[])
      >- (qexists_tac `v` >> rw[fAND_def,feval_def,APPLY_UPDATE_THM] (* 3 *)
         >- fs[mm2folm_def]
-	>- (fs[interpret_def,APPLY_UPDATE_THM] >> rw[mm2folm_def])
+	>- (fs[termval_def,APPLY_UPDATE_THM] >> rw[mm2folm_def])
 	>- (`((x + 1 =+ v) σ) (x + 1) = v` by rw[APPLY_UPDATE_THM] >>
            `IMAGE ((x + 1 =+ v) σ) 𝕌(:num) ⊆ M.frame.world`
 	   by (rw[IMAGE_DEF,SUBSET_DEF] >> Cases_on `x'' = x + 1` (* 2 *)
@@ -127,17 +97,18 @@ val prop_2_47_i = store_thm(
 	   `() = u` by fs[] >>
            metis_tac[fsatis_def]))
      >- (fs[SUBSET_DEF,IMAGE_DEF,mm2folm_def] >> metis_tac[])
-     >- (qexists_tac `x'` >> rw[] (* 3 *)
-        >- fs[feval_def,fAND_def,fsatis_def,interpret_def,APPLY_UPDATE_THM,mm2folm_def]
+     >- (qexists_tac `a` >> rw[] (* 3 *)
+        >- fs[feval_def,fAND_def,fsatis_def,termval_def,APPLY_UPDATE_THM,mm2folm_def]
 	>- fs[mm2folm_def]
 	>- (fs[feval_def,fAND_def,fsatis_def] >>
-	   `IMAGE ((x + 1 =+ x') σ) 𝕌(:num) ⊆ M.frame.world`
-	   by (rw[IMAGE_DEF,SUBSET_DEF] >> Cases_on `x''' = x + 1` (* 2 *)
+	   `IMAGE ((x + 1 =+ a) σ) 𝕌(:num) ⊆ M.frame.world`
+	   by (rw[IMAGE_DEF,SUBSET_DEF] >> Cases_on `x'' = x + 1` (* 2 *)
 	      >- (rw[APPLY_UPDATE_THM] >> fs[mm2folm_def])
 	      >- (rw[APPLY_UPDATE_THM] >> fs[IMAGE_DEF,SUBSET_DEF] >> metis_tac[])) >>
-	   `((x + 1 =+ x') σ) (x + 1) = x'` by fs[APPLY_UPDATE_THM] >>
-	   `(mm2folm M).domain = M.frame.world` by fs[mm2folm_def] >>
-	   metis_tac[]))));
+	   `((x + 1 =+ a) σ) (x + 1) = a` by fs[APPLY_UPDATE_THM] >>
+	   `(mm2folm M).Dom = M.frame.world` by fs[mm2folm_def] >>
+	   first_x_assum (qspecl_then [`M`,`σ(|x+1|->a|)`,`x+1`] mp_tac) >>
+           rw[APPLY_UPDATE_THM]))));
 
 
 
@@ -147,11 +118,11 @@ val fFORALL_def = Define`
 
 val prop_2_47_ii = store_thm(
   "prop_2_47_ii",
-  ``!phi M. universal_true M phi <=> (!σ. IMAGE σ univ(:num) SUBSET M.frame.world ==> (fsatis (mm2folm M) σ (fFORALL x (ST x u phi))))``,
+  ``!phi M. universal_true M phi <=> (!σ. IMAGE σ univ(:num) SUBSET M.frame.world ==> (fsatis (mm2folm M) σ (fFORALL x (ST x phi))))``,
   rw[universal_true_def,fFORALL_def,fsatis_def,feval_def] >> rw[EQ_IMP_THM] (* 3 *)
-  >- fs[mm2folm_def]
-  >- (`!x'. x' IN (mm2folm M).domain ==> feval (mm2folm M) ((x =+ x') σ) (ST x () phi)` suffices_by metis_tac[] >> rw[] >>
-     `fsatis (mm2folm M) ((x =+ x') σ) (ST x () phi)` suffices_by metis_tac[fsatis_def] >>
+  >- (fs[mm2folm_def,valuation_def,IMAGE_DEF,SUBSET_DEF] >> metis_tac[])
+  >- (`!x'. x' IN (mm2folm M).Dom ==> feval (mm2folm M) ((x =+ x') σ) (ST x phi)` suffices_by metis_tac[] >> rw[] >>
+     `fsatis (mm2folm M) ((x =+ x') σ) (ST x phi)` suffices_by metis_tac[fsatis_def] >>
      `x' IN M.frame.world` by fs[mm2folm_def] >>
      `satis M x' phi` by metis_tac[] >>
      `IMAGE ((x =+ x') σ) 𝕌(:num) ⊆ M.frame.world`
@@ -160,13 +131,13 @@ val prop_2_47_ii = store_thm(
   >- (`IMAGE (\n.w) 𝕌(:num) ⊆ M.frame.world`
          by (rw[IMAGE_DEF,SUBSET_DEF] >> metis_tac[]) >>
      `∀x'.
-            x' IN (mm2folm M).domain ==>
-            feval (mm2folm M) ((x =+ x') (\n.w)) (ST x () phi)` by metis_tac[] >>
-     `w IN (mm2folm M).domain` by fs[mm2folm_def] >>
-     `feval (mm2folm M) ((x =+ w) (λn. w)) (ST x () phi)` by metis_tac[] >>
+            x' IN (mm2folm M).Dom ==>
+            feval (mm2folm M) ((x =+ x') (\n.w)) (ST x phi)` by metis_tac[] >>
+     `w IN (mm2folm M).Dom` by fs[mm2folm_def] >>
+     `feval (mm2folm M) ((x =+ w) (λn. w)) (ST x phi)` by metis_tac[] >>
      `IMAGE ((x =+ w) (λn. w)) 𝕌(:num) ⊆ M.frame.world`
          by (rw[IMAGE_DEF,SUBSET_DEF] >> Cases_on `x'' = x` >> rw[APPLY_UPDATE_THM]) >>
-     `fsatis (mm2folm M) ((x =+ w) (λn. w)) (ST x () phi)` by metis_tac[fsatis_def] >>
+     `fsatis (mm2folm M) ((x =+ w) (λn. w)) (ST x phi)` by metis_tac[fsatis_def] >>
      `((x =+ w) (λn. w)) x = w` by fs[APPLY_UPDATE_THM] >>
      imp_res_tac prop_2_47_i >> metis_tac[]));
      
@@ -174,49 +145,42 @@ val prop_2_47_ii = store_thm(
 
 
 val ST_alt_def = Define`
-  (ST_alt x u (VAR p) <=> fPrel p (fVar x)) /\
-  (ST_alt x u (FALSE) <=> fNOT (fEQ (fVar x) (fVar x))) /\
-  (ST_alt x u (NOT phi) <=> fNOT (ST_alt x u phi)) /\
-  (ST_alt x u (DISJ phi psi) <=> fDISJ (ST_alt x u phi) (ST_alt x u psi)) /\
-  (ST_alt x u (DIAM phi) <=> fEXISTS (1 - x) (fAND (fRrel u (fVar x) (fVar (1 - x))) (ST_alt (1 - x) u phi)))`;
+  (ST_alt x (VAR p) = fP p (fV x)) /\
+  (ST_alt x (FALSE) = fFALSE) /\
+  (ST_alt x (NOT phi) = fNOT (ST_alt x phi)) /\
+  (ST_alt x (DISJ phi psi) = fDISJ (ST_alt x phi) (ST_alt x psi)) /\
+  (ST_alt x (DIAM phi) = fEXISTS (1 - x) (fAND (fR (fV x) (fV (1 - x))) (ST_alt (1 - x) phi)))`;
 
 
 val prop_2_47_i_alt = store_thm(
   "prop_2_47_i_alt",
   ``!M w:'b phi σ. (IMAGE σ univ(:num)) SUBSET M.frame.world
-                       ==> (satis M (σ 1) phi <=> fsatis (mm2folm M) σ (ST_alt 1 u phi)) /\
-		           (satis M (σ 0) phi <=> fsatis (mm2folm M) σ (ST_alt 0 u phi))``,
+                       ==> (satis M (σ 1) phi <=> fsatis (mm2folm M) σ (ST_alt 1 phi)) /\
+		           (satis M (σ 0) phi <=> fsatis (mm2folm M) σ (ST_alt 0 phi))``,
   Induct_on `phi` >> rw[] (* 10 *)
   >- (rw[feval_def,ST_alt_def,fsatis_def] >> eq_tac >> rw[] (* 3 *)
-     >- rw[mm2folm_def]
-     >- (rw[mm2folm_def,interpret_def] (* 2 *)
+     >- (fs[mm2folm_def,valuation_def,IMAGE_DEF,SUBSET_DEF] >> metis_tac[])
+     >- (rw[mm2folm_def,termval_def] (* 2 *)
         >> metis_tac[satis_def,IN_DEF])
-     >- (fs[mm2folm_def,interpret_def] >> rw[satis_def] >> metis_tac[IN_DEF]))
-  >- (rw[feval_def,ST_alt_def,fsatis_def,mm2folm_def,interpret_def] >> eq_tac >> rw[] (* 3 *)
+     >- (fs[mm2folm_def,termval_def] >> rw[satis_def] >> metis_tac[IN_DEF]))
+  >- (rw[feval_def,ST_alt_def,fsatis_def,mm2folm_def,termval_def] >> eq_tac >> rw[] (* 4 *)
+     >- (fs[mm2folm_def,valuation_def,IMAGE_DEF,SUBSET_DEF] >> metis_tac[])
      >- metis_tac[satis_def,IN_DEF]
      >- metis_tac[satis_def,IN_DEF]
      >- (rw[satis_def] >> metis_tac[IN_DEF]))
-  >- (fs[satis_def,feval_def,ST_alt_def,fsatis_def,mm2folm_def,interpret_def])
-  >- (fs[satis_def,feval_def,ST_alt_def,fsatis_def,mm2folm_def,interpret_def])
-  >- (fs[satis_def,feval_def,ST_alt_def,fsatis_def,mm2folm_def,interpret_def])
-  >- (fs[satis_def,feval_def,ST_alt_def,fsatis_def,mm2folm_def,interpret_def])
-  >- (rw[satis_def,feval_def,ST_alt_def,fsatis_def] >> eq_tac >> rw[] (* 5 *)
-     >- fs[mm2folm_def]
-     >- fs[mm2folm_def]
-     >- fs[mm2folm_def]
-     >- fs[]
-     >- (fs[IMAGE_DEF,SUBSET_DEF] >> metis_tac[]))
-  >- (rw[satis_def,feval_def,ST_alt_def,fsatis_def] >> eq_tac >> rw[] (* 5 *)
-     >- fs[mm2folm_def]
-     >- fs[mm2folm_def]
-     >- fs[mm2folm_def]
-     >- fs[mm2folm_def]
-     >- (fs[IMAGE_DEF,SUBSET_DEF] >> metis_tac[]))
+  >- (fs[satis_def,feval_def,ST_alt_def,fsatis_def,mm2folm_def,termval_def,valuation_def,IMAGE_DEF,SUBSET_DEF] >> metis_tac[])
+  >- (fs[satis_def,feval_def,ST_alt_def,fsatis_def,mm2folm_def,termval_def,valuation_def,IMAGE_DEF,SUBSET_DEF] >> metis_tac[])
+  >- (fs[satis_def,feval_def,ST_alt_def,fsatis_def,mm2folm_def,termval_def,valuation_def,IMAGE_DEF,SUBSET_DEF] >> metis_tac[])
+  >- (fs[satis_def,feval_def,ST_alt_def,fsatis_def,mm2folm_def,termval_def,valuation_def,IMAGE_DEF,SUBSET_DEF] >> metis_tac[])
+  >- (rw[satis_def,feval_def,ST_alt_def,fsatis_def] >> eq_tac >> rw[] (* 5 *) >>
+     fs[mm2folm_def,valuation_def,IMAGE_DEF,SUBSET_DEF] >> metis_tac[])
+  >- (rw[satis_def,feval_def,ST_alt_def,fsatis_def] >> eq_tac >> rw[] (* 5 *) >>
+     fs[mm2folm_def,valuation_def,IMAGE_DEF,SUBSET_DEF] >> metis_tac[])
   >- (rw[satis_def,feval_def,ST_alt_def,fsatis_def] >> eq_tac >> rw[] (* 4 *)
-     >- fs[mm2folm_def]
+     >- (fs[mm2folm_def,valuation_def,IMAGE_DEF,SUBSET_DEF] >> metis_tac[])
      >- (qexists_tac `v` >> rw[fAND_def,feval_def,APPLY_UPDATE_THM] (* 3 *)
-        >- fs[mm2folm_def]
-	>- rw[mm2folm_def,interpret_def,APPLY_UPDATE_THM] 
+        >- (fs[mm2folm_def,valuation_def,IMAGE_DEF,SUBSET_DEF] >> metis_tac[])
+	>- rw[mm2folm_def,termval_def,APPLY_UPDATE_THM] 
 	>- (fs[fsatis_def] >>
            `((0 =+ v) σ) 0 = v` by rw[APPLY_UPDATE_THM] >>
            `IMAGE ((0 =+ v) σ) 𝕌(:num) ⊆ M.frame.world`
@@ -224,21 +188,22 @@ val prop_2_47_i_alt = store_thm(
 	           >> rw[APPLY_UPDATE_THM] >> fs[IMAGE_DEF,SUBSET_DEF] >> metis_tac[]) >>
 	   metis_tac[]))
      >- (fs[SUBSET_DEF,IMAGE_DEF] >> metis_tac[])
-     >- (qexists_tac `x` >> rw[] (* 3 *)
-        >- fs[feval_def,fAND_def,fsatis_def,mm2folm_def,interpret_def,APPLY_UPDATE_THM]
+     >- (qexists_tac `a` >> rw[] (* 3 *)
+        >- fs[feval_def,fAND_def,fsatis_def,mm2folm_def,termval_def,APPLY_UPDATE_THM]
         >- fs[mm2folm_def]
 	>- (fs[feval_def,fAND_def,fsatis_def] >>
-	   `IMAGE ((0 =+ x) σ) 𝕌(:num) ⊆ M.frame.world`
-	   by (rw[IMAGE_DEF,SUBSET_DEF] >> Cases_on `x'' = 0` (* 2 *)
+	   `IMAGE ((0 =+ a) σ) 𝕌(:num) ⊆ M.frame.world`
+	   by (rw[IMAGE_DEF,SUBSET_DEF] >> Cases_on `x' = 0` (* 2 *)
 	      >> rw[APPLY_UPDATE_THM] >> fs[IMAGE_DEF,SUBSET_DEF,mm2folm_def] >> metis_tac[]) >>
-	   `((0 =+ x) σ) 0 = x` by fs[APPLY_UPDATE_THM] >>
-	   `IMAGE ((0 =+ x) σ) 𝕌(:num) ⊆ (mm2folm M).domain` by fs[mm2folm_def] >>
-	   metis_tac[mm2folm_def])))
+	   `((0 =+ a) σ) 0 = a` by fs[APPLY_UPDATE_THM] >>
+	   `IMAGE ((0 =+ a) σ) 𝕌(:num) ⊆ (mm2folm M).Dom` by fs[mm2folm_def] >>
+	   first_x_assum (qspecl_then [`M`,`σ(|0|->a|)`] mp_tac) >> 
+           rw[APPLY_UPDATE_THM])))
   >- (rw[satis_def,feval_def,ST_alt_def,fsatis_def] >> eq_tac >> rw[] (* 4 *)
-     >- fs[mm2folm_def]
+     >- (fs[mm2folm_def,valuation_def,IMAGE_DEF,SUBSET_DEF] >> metis_tac[])
      >- (qexists_tac `v` >> rw[fAND_def,feval_def,APPLY_UPDATE_THM] (* 3 *)
         >- fs[mm2folm_def]
-	>- rw[mm2folm_def,interpret_def,APPLY_UPDATE_THM] 
+	>- rw[mm2folm_def,termval_def,APPLY_UPDATE_THM] 
         >- (fs[fsatis_def] >>
            `((1 =+ v) σ) 1= v` by rw[APPLY_UPDATE_THM] >>
            `IMAGE ((1 =+ v) σ) 𝕌(:num) ⊆ M.frame.world`
@@ -246,22 +211,24 @@ val prop_2_47_i_alt = store_thm(
 	          >> rw[APPLY_UPDATE_THM] >> fs[IMAGE_DEF,SUBSET_DEF] >> metis_tac[]) >>
            metis_tac[]))
      >- (fs[SUBSET_DEF,IMAGE_DEF] >> metis_tac[])
-     >- (qexists_tac `x` >> rw[] (* 3 *)
-        >- fs[feval_def,fAND_def,fsatis_def,mm2folm_def,interpret_def,APPLY_UPDATE_THM]
+     >- (qexists_tac `a` >> rw[] (* 3 *)
+        >- fs[feval_def,fAND_def,fsatis_def,mm2folm_def,termval_def,APPLY_UPDATE_THM]
         >- fs[mm2folm_def]
         >- (fs[feval_def,fAND_def,fsatis_def] >>
-	   `IMAGE ((1 =+ x) σ) 𝕌(:num) ⊆ M.frame.world`
+	   `IMAGE ((1 =+ a) σ) 𝕌(:num) ⊆ M.frame.world`
 	   by (rw[IMAGE_DEF,SUBSET_DEF] >> Cases_on `x'' = 0` (* 2 *)
 	      >> rw[APPLY_UPDATE_THM] >> fs[IMAGE_DEF,SUBSET_DEF,mm2folm_def] >> metis_tac[]) >>
-	   `((1 =+ x) σ) 1 = x` by fs[APPLY_UPDATE_THM] >>
-	   `IMAGE ((1 =+ x) σ) 𝕌(:num) ⊆ (mm2folm M).domain` by fs[mm2folm_def] >>
-	   metis_tac[mm2folm_def]))));
+	   `((1 =+ a) σ) 1 = a` by fs[APPLY_UPDATE_THM] >>
+	   `IMAGE ((1 =+ a) σ) 𝕌(:num) ⊆ (mm2folm M).Dom` by fs[mm2folm_def] >>
+	   first_x_assum (qspecl_then [`M`,`σ(|1|->a|)`] mp_tac) >> 
+           rw[APPLY_UPDATE_THM]))));
 
 
 val ST_alt_two_var = store_thm(
   "ST_alt_two_var",
-  ``!phi. fvars (ST_alt 0 u phi) SUBSET {0;1} /\ fvars (ST_alt 1 u phi) SUBSET {0;1}``,
-  Induct_on `phi` >> rw[] >> fs[ST_alt_def,fvars_def,SUBSET_DEF,tvars_def] >> rw[]
+  ``!phi. FV (ST_alt 0 phi) SUBSET {0;1} /\ FV (ST_alt 1 phi) SUBSET {0;1}``,
+  Induct_on `phi` >> rw[] >> fs[ST_alt_def,FV_def,SUBSET_DEF,FVT_def] >> 
+   rw[FV_def]
   >- metis_tac[]
   >- metis_tac[]
   >- metis_tac[]
@@ -274,7 +241,11 @@ val ST_alt_two_var = store_thm(
 
 
 val fequiv_def = Define`
-  fequiv (μ:'b itself) ff1 ff2 <=> (!M (σ:num -> 'b). (IMAGE σ univ(:num)) SUBSET M.frame.world
+  fequiv (μ:'b itself) ff1 ff2 <=>
+
+
+
+ (!M (σ:num -> 'b). (IMAGE σ univ(:num)) SUBSET M.frame.world
                                                         ==> (fsatis (mm2folm M) σ ff1 <=> fsatis (mm2folm M) σ ff2))`;
 
 
